Projects/AP/Alts/Alt1/Equiv.lean
@@ -16,6 +16,8 @@ theorem ofAlt_dist {p₁ p₂ : PointZ} :
 dist (.ofAlt p₁) (.ofAlt p₂) = (p₁.dist p₂).toNat := by
   rcases p₁, p₂ with ⟨⟨x₁, y₁⟩, ⟨x₂, y₂⟩⟩; simp [dist]
 
+@[simp] theorem Game.act_iff {pw} {g : Game pw} : g.act ↔ g.s.act := by rfl
+
 @[simp]
 theorem Board.pw_toAlt {b : Board} {pw aTurn hist} : (b.toAlt pw aTurn hist).pw = pw := rfl
 
@@ -190,7 +192,7 @@ theorem Game.play_zero {pw} {g : Game pw} : g.play 0 = g := rfl
 theorem Game.s_initGame {pw a d s} : (initGame a d s : Game pw).s = s := rfl
 
 @[simp]
-theorem Game.act_initGame {pw a d s} : (initGame a d s : Game pw).act = s.act := rfl
+theorem Game.act_initGame {pw a d s} : (initGame a d s : Game pw).s.act = s.act := rfl
 
 @[simp]
 theorem act_state₀ : state₀.act := trivial
@@ -207,19 +209,22 @@ theorem Game.play_succ' {pw} {g : Game pw} {n} : g.play (n + 1) = g.playMove.pla
 theorem Game.state_setState {pw} {g : Game pw} {s} : (g.setState s).s = s := rfl
 
 @[simp]
-theorem Game.act_setState {pw} {g : Game pw} {s} : (g.setState s).act ↔ s.act := by rfl
+theorem Game.act_setState {pw} {g : Game pw} {s} : (g.setState s).s.act ↔ s.act := by rfl
 
 @[simp]
 theorem Game.act_applyDMove {s m} : (applyDMove s m).act ↔ s.act := by rfl
 
 @[simp]
-theorem Game.act_playDMoveAt {pw} {g : Game pw} {h} : (playDMoveAt g h).act := by
+theorem Game.act_playDMoveAt {pw} {g : Game pw} {h} : (playDMoveAt g h).s.act := by
   simpa [playDMoveAt]
 
-theorem Game.playMove_eq_of_not_act {pw} {g : Game pw} (h : ¬g.act) : g.playMove = g := by
-  simp [playMove, h]
+theorem Game.playMove_eq {pw} {g : Game pw} : g.playMove = haveI := Classical.propDecidable
+if hs : g.s.act then playAMoveAt # playDMoveAt g hs else g := rfl
 
-theorem Game.play_eq_of_not_act {pw} {g : Game pw} {n} (h : ¬g.act) : g.play n = g := by
+theorem Game.playMove_eq_of_not_act {pw} {g : Game pw} (h : ¬g.s.act) : g.playMove = g := by
+  simp [playMove_eq, h]
+
+theorem Game.play_eq_of_not_act {pw} {g : Game pw} {n} (h : ¬g.s.act) : g.play n = g := by
   induction n; rfl; nm n ih; rw [play_succ, ih]; exact playMove_eq_of_not_act h
 
 @[simp]
@@ -227,7 +232,7 @@ theorem State.act_finish {s : State} : ¬s.finish.act := by
   simp [finish]
 
 @[simp]
-theorem Game.act_finish {pw} {g : Game pw} : ¬g.finish.act := by
+theorem Game.act_finish {pw} {g : Game pw} : ¬g.finish.s.act := by
   simp [finish]
 
 @[simp]
@@ -303,714 +308,980 @@ theorem State.act_applyAMove {s : State} {b} : (applyAMove s b).act ↔ s.act :=
 theorem State.aTurn_applyAMove {s : State} {b} : (applyAMove s b).aTurn = !s.aTurn := by
   simp [applyAMove]
 
-theorem Game.act_play_initGame_of_not_aTurn {pw a d n g s}
-(h₁ : s.aTurn = false) (h₂ : s.act) (h₃ : (initGame a d s : Game pw).play n = g)
-(h₄ : g.s.aTurn = false) : g.act := by
-  induction n generalizing s g
-  · simp at h₃; simpa [←h₃]
-  nm n ih
-  rw [play_succ'] at h₃
-  simp [playMove, h₂] at h₃
-  simp [playDMoveAt] at h₃
-  generalize_proofs at h₃
-  generalize h₅ : applyDMove s (d.f s h₂).m = s₁ at h₃
-  have h₆ : s₁.act; simpa [←h₅]
-  simp [playAMoveAt] at h₃
-  rw! (castMode := .all) [eq_true_of h₆, true_and] at h₃
-  split_ifs at h₃ with h₇
-  rotate_left
-  · replace h₃ := congrArg (·.s.aTurn) h₃
-    simp [←h₅, h₁, h₄] at h₃
-  simp [playAMoveAt'] at h₃
-  generalize_proofs at h₃
-  generalize hs₂ : applyAMove s₁ (a.f s₁ h₆ h₇).m = s₂ at h₃
-  have H₁ : s₂.act; simpa [←hs₂]
-  have H₂ : s₁.aTurn = true; simpa [←h₅]
-  have H₃ : s₂.aTurn = false; simpa [←hs₂]
-  grind
-
-@[simp]
-theorem Game.s_playAMoveAt'_eq_iff {pw} {g₁ g₂ : Game pw} {h₁ h₂ h₃ h₄} :
-(playAMoveAt' g₁.a g₁ h₁ h₂).s = (playAMoveAt' g₂.a g₂ h₃ h₄).s ↔
-applyAMove g₁.s (g₁.a.f g₁.s h₁ h₂).m = applyAMove g₂.s (g₂.a.f g₂.s h₃ h₄).m := by rfl
-
-@[simp]
-theorem Game.s_playDMoveAt_eq_iff {pw} {g₁ g₂ : Game pw} {h₁ h₂} :
-(playDMoveAt g₁ h₁).s = (playDMoveAt g₂ h₂).s ↔
-applyDMove g₁.s (g₁.d.f g₁.s h₁).m = applyDMove g₂.s (g₂.d.f g₂.s h₂).m := by rfl
-
-@[simp] theorem Game.a_finish {pw} {g : Game pw} : g.finish.a = g.a := rfl
-@[simp] theorem Game.d_finish {pw} {g : Game pw} : g.finish.d = g.d := rfl
-
-@[simp] theorem Game.a_setState {pw} {g : Game pw} {s} : (g.setState s).a = g.a := rfl
-@[simp] theorem Game.d_setState {pw} {g : Game pw} {s} : (g.setState s).d = g.d := rfl
-
-@[simp]
-theorem Game.a_playAMoveAt' {pw} {g : Game pw} {a : A pw} {h₁ h₂} :
-(playAMoveAt' a g h₁ h₂).a = g.a := rfl
-
-@[simp]
-theorem Game.d_playAMoveAt' {pw} {g : Game pw} {a : A pw} {h₁ h₂} :
-(playAMoveAt' a g h₁ h₂).d = g.d := rfl
-
-@[simp]
-theorem Game.a_playAMoveAt {pw} {g : Game pw} : (playAMoveAt g).a = g.a := by
-  simp [playAMoveAt]; split_ifs <;> simp
-
-@[simp]
-theorem Game.d_playAMoveAt {pw} {g : Game pw} : (playAMoveAt g).d = g.d := by
-  simp [playAMoveAt]; split_ifs <;> simp
-
-@[simp]
-theorem Game.a_playDMoveAt {pw} {g : Game pw} {h} : (playDMoveAt g h).a = g.a := by
-  simp [playDMoveAt]
-
-@[simp]
-theorem Game.d_playDMoveAt {pw} {g : Game pw} {h} : (playDMoveAt g h).d = g.d := by
-  simp [playDMoveAt]
-
-@[simp]
-theorem Game.a_playMove {pw} {g : Game pw} : g.playMove.a = g.a := by
-  simp [playMove]; split_ifs <;> simp
-
-@[simp]
-theorem Game.d_playMove {pw} {g : Game pw} : g.playMove.d = g.d := by
-  simp [playMove]; split_ifs <;> simp
-
-@[simp]
-theorem Game.a_play {pw} {g : Game pw} {n} : (g.play n).a = g.a := by
-  induction n; rfl; simpa [play_succ]
-
-@[simp]
-theorem Game.d_play {pw} {g : Game pw} {n} : (g.play n).d = g.d := by
-  induction n; rfl; simpa [play_succ]
-
-@[simp]
-theorem State.board_finish {s : State} : s.finish.board = s.board := rfl
-
-theorem Game.s_playAMoveAt_eq_iff_of {pw} {g₁ g₂ : Game pw} (h₁ : g₁.s.act ↔ g₂.s.act)
-(h₂ : AHasValidMove pw g₁.s.board ↔ AHasValidMove pw g₂.s.board) : ∀ h₁ h₂ h₃ h₄,
-(playAMoveAt g₁).s = (playAMoveAt g₂).s ↔
-applyAMove g₁.s (g₁.a.f g₁.s h₁ h₂).m = applyAMove g₂.s (g₂.a.f g₂.s h₃ h₄).m := by
-  simp_all [playAMoveAt, playAMoveAt', applyAMove, act]
-
-theorem Game.playAMoveAt_eq_of_neg {pw} {g : Game pw}
-(h : ¬g.act ∨ ¬AHasValidMove pw g.s.board) : playAMoveAt g = g.finish := by
-  simp [playAMoveAt]; tauto
-
-theorem Game.s_play_initGame_d_set_eq_of_ne {pw a d s s₁ dRef n}
-(h : ∀ k < n, (initGame a d s |>.play k : Game pw).s ≠ s₁) :
-(initGame a (d.set s₁ dRef) s |>.play n).s = (initGame a d s |>.play n).s := by
-  induction n; simp
-  nm n ih
-  specialize ih # by grind
-  simp [play_succ, playMove, act]
-  rw! (castMode := .all) [ih]
-  split_ifs with h₁
-  on_goal 2 => exact ih
-  generalize hg : (initGame a d s).play n = g at *
-  generalize hg₁ : (initGame a (d.set s₁ dRef) s).play n = g₁ at *
-  have H₁ : g₁.a = g.a; simp [←hg, ←hg₁]
-  simp [playDMoveAt]
-  rw! [ih]
-  have h₂ : applyDMove g.s (g₁.d.f g.s h₁).m = applyDMove g.s (g.d.f g.s h₁).m
-  · congr 2; simp [←hg₁, D.set]
-    rw [if_neg]; simp [←hg]
-    rw [←hg]; apply h; omega
-  rw [h₂]
-  generalize h₃ : applyDMove g.s (g.d.f g.s h₁).m = s'
-  have h₄ : s'.act; simpa [←h₃]
-  by_cases h₅ : ¬AHasValidMove pw s'.board
-  · iterate 2 rw [playAMoveAt_eq_of_neg # by tauto];; simp
-  push Not at h₅
-  have h₆ := @s_playAMoveAt_eq_iff_of _ (g₁.setState s') (g.setState s')
-    (by simp) (by simp) (by simpa) (by simpa) (by simpa) (by simpa)
-  rw [h₆]; clear h₆
-  simp; grind
-
-theorem Game.act_of_act_playMove {pw} {g : Game pw} (h : g.playMove.act) : g.act := by
-  by_contra h₁; simp [playMove, h₁] at h
-
-theorem Game.act_of_act_play {pw} {g : Game pw} {n} (h : (g.play n).act) : g.act := by
-  induction n; simp at h; exact h
-  nm n ih; apply ih
-  simp [play_succ] at h
-  exact act_of_act_playMove h
-
-@[simp]
-theorem State.length_history_applyAMove {s m} :
-(applyAMove s m).history.length = s.history.length + 1 := by
-  simp [applyAMove]
-
-@[simp]
-theorem State.length_history_applyDMove {s m} :
-(applyDMove s m).history.length = s.history.length + 1 := by
-  simp [applyDMove]
-
-@[simp]
-theorem Game.length_history_playAMoveAt' {pw} {g : Game pw} {a : A pw} {h₁ h₂} :
-(playAMoveAt' a g h₁ h₂).s.history.length = g.s.history.length + 1 := by
-  simp [playAMoveAt']
-
-@[simp]
-theorem Game.length_history_playDMoveAt {pw} {g : Game pw} {h} :
-(playDMoveAt g h).s.history.length = g.s.history.length + 1 := by
-  simp [playDMoveAt]
-
-@[simp]
-theorem State.history_finish {s : State} : s.finish.history = s.history := rfl
-
-theorem Game.length_history_playMove_eq_of_act {pw} {g : Game pw}
-(h : g.playMove.act) : g.playMove.s.history.length = g.s.history.length + 2 := by
-  have h₁ := act_of_act_playMove h
-  simp [h₁, playMove, playAMoveAt]
-  rw! (castMode := .all) [eq_true_of act_playDMoveAt, true_and]
-  rw [dif_pos]; simp
-  simp [playMove, h₁, playAMoveAt] at h
-  split_ifs at h with h₂ <;> simp_all
-
-theorem Game.length_history_play_eq_of_act {pw} {g : Game pw} {n}
-(h : (g.play n).act) : (g.play n).s.history.length = g.s.history.length + n * 2 := by
-  induction n; simp; nm n ih
-  simp [play_succ] at h ⊢
-  specialize ih # act_of_act_playMove h
-  rw [length_history_playMove_eq_of_act h]; omega
-
-@[simp]
-theorem Game.play_add {pw} {g : Game pw} {n m} : g.play (n + m) = (g.play n).play m := by
-  nth_rw 1 [play, add_comm]; rw [Function.iterate_add]; rfl
-
-theorem Game.s_play_eq_iff_of_act {pw} {g : Game pw} {n m}
-(h : g.play (max n m) |>.act) : (g.play n).s = (g.play m).s ↔ n = m := by
-  symm; constructor; rintro rfl; rfl
-  contrapose!
-  intro h₁
-  apply ne_of_congr (·.history.length)
-  wlog h₂ : n < m with ih; grind
-  clear h₁
-  rw [max_eq_right_of_lt h₂] at h
-  obtain ⟨m, rfl⟩ := Nat.exists_eq_add_of_le # le_of_lt h₂
-  simp at h ⊢
-  rw [length_history_play_eq_of_act h]; omega
-
-@[simp]
-theorem history_state₀ : state₀.history = [] := rfl
-
-@[simp]
-theorem Game.aTurn_playAMoveAt' {pw} {g : Game pw} {a : A pw} {h₁ h₂} :
-(playAMoveAt' a g h₁ h₂).s.aTurn = !g.s.aTurn := by
-  simp [playAMoveAt']
-
-theorem Game.aTurn_playMove_eq_of_act {pw} {g : Game pw}
-(h : g.playMove.act) : g.playMove.s.aTurn = g.s.aTurn := by
-  simp [playMove] at h ⊢
-  split_ifs at h ⊢ with h₁; on_goal 2 => contradiction
-  generalize hg₁ : playDMoveAt g h₁ = g₁ at h ⊢
-  have h₂ : g₁.act; simp [←hg₁]
-  simp [playAMoveAt] at h ⊢
-  rw! (castMode := .all) [eq_true_of h₂, true_and] at h ⊢
-  split_ifs at h ⊢ with h₃; on_goal 2 => simp at h
-  simp [←hg₁]
-
-theorem Game.aTurn_play_eq_of_act {pw} {g : Game pw} {n}
-(h : (g.play n).act) : (g.play n).s.aTurn = g.s.aTurn := by
-  induction n; simp; nm n ih; simp at h ⊢
-  specialize ih (act_of_act_playMove h)
-  rwa [aTurn_playMove_eq_of_act h]
-
-theorem aState_iff {pw s} : AState pw s ↔ s.WF pw ∧ s.aTurn = true := by
-  constructor <;> rintro ⟨⟩ <;> constructor <;> assumption
-
-theorem dState_iff {pw s} : DState pw s ↔ s.WF pw ∧ s.aTurn = false := by
-  constructor <;> rintro ⟨⟩ <;> constructor <;> assumption
-
-@[simp, instance]
-theorem aState_playDMoveAt {pw} {g : Game pw} {h}
-[hs : DState pw g.s] : AState pw (playDMoveAt g h).s := by
-  rw [dState_iff] at hs; choose hs ht using hs; rw [aState_iff]
-  rw [State.wf_iff] at hs ⊢
-  symm; split_ands; simpa
-  choose a d n g₁ h₁ h₂ using hs
-  symm at h₂; rcases h₂ with ⟨h', h₂⟩ | h₂
-  · contrapose h₂; clear h₂
-    apply ne_of_congr (·.aTurn)
-    simp [ht]
-    rw [←h₁] at h' ⊢
-    simp [Game.aTurn_play_eq_of_act h']
-  have h₃ : g₁.s.act
-  · replace h₂ := congrArg (·.aTurn) h₂
-    simp [ht] at h₂
-    apply Game.act_play_initGame_of_not_aTurn _ _ h₁ <;> simp_all
-  generalize hg' : (initGame a (d.set g₁.s g.d) state₀).play n = g'
-  refine' ⟨a, _, n, g', hg', _⟩; right
-  have h₄ : g'.s = g.s
-  · rw [←h₂, ←h₁, ←hg']
-    apply Game.s_play_initGame_d_set_eq_of_ne
-    intro k hk
-    simp [←h₁]
-    rw [Game.s_play_eq_iff_of_act]; omega
-    rw [max_eq_right_of_lt hk, h₁]
-    exact h₃
-  simp [h₄, h, applyDMove, applyMove]
-  congr 1; simp [←hg', D.set]; grind
-
-theorem Game.playAMoveAt_eq_of_not_act {pw} {g : Game pw}
-(h : ¬g.act) : playAMoveAt g = g.finish := by
-  simp [playAMoveAt, h]
-
-theorem Game.s_play_initGame_a_set_eq_of_ne {pw a d s s₁ aRef n}
-(h : ∀ k < n, ∀ h, (playDMoveAt (initGame a d s |>.play k) h : Game pw).s ≠ s₁) :
-(initGame (a.set s₁ aRef) d s |>.play n).s = (initGame a d s |>.play n).s := by
-  induction n; simp
-  nm n ih
-  specialize ih # by grind
-  simp [play_succ, playMove, act]
-  rw! (castMode := .all) [ih]
-  split_ifs with h₁
-  on_goal 2 => exact ih
-  generalize hg : (initGame a d s).play n = g at *
-  generalize hg₁ : (initGame (a.set s₁ aRef) d s).play n = g₁ at *
-  generalize_proofs H₁
-  generalize hgx : playDMoveAt g₁ H₁ = gx
-  generalize hgy : playDMoveAt g h₁ = gy
-  have H₂ : gx.s = gy.s
-  · subst hgx hgy
-    simp
-    congr 1
-    simp [←hg₁, ←hg]
-    rw! [ih]
-    rfl
-  simp [playAMoveAt, act]
-  rw! (castMode := .all) [H₂]
-  split_ifs with H₃; on_goal 2 => simp [H₂]
-  rcases H₃ with ⟨H₃, H₄⟩
-  simp
-  have H₅ : gx.a = a.set s₁ aRef; simp [←hgx, ←hg₁]
-  have H₆ : gy.a = a; simp [←hgy, ←hg]
-  rw! [H₅, H₆, ←H₂]
-  congr 2
-  simp [A.set]
-  contrapose!; rintro - rfl
-  contrapose h; clear h
-  simp
-  use n, by rfl
-  simp [hg, h₁, hgy, H₂]
-
-theorem Game.playAMoveAt_eq_of_pos {pw} {g : Game pw}
-(h₁ : g.act) (h₂ : AHasValidMove pw g.s.board) :
-playAMoveAt g = playAMoveAt' g.a g h₁ h₂ := by
-  simp [playAMoveAt, h₁, h₂]
-
-theorem Game.act_of_act_playAMoveAt {pw} {g : Game pw} (h : playAMoveAt g |>.act) : g.act := by
-  by_contra! h₁; simp [playAMoveAt, h₁] at h
-
-theorem Game.aHasValidMove_of_act_playAMoveAt {pw} {g : Game pw}
-(h : playAMoveAt g |>.act) : AHasValidMove pw g.s.board := by
-  by_contra! h₁; simp [playAMoveAt, h₁] at h
-
-theorem Game.s_playAMoveAt_eq_iff_of_act_playAMoveAt {pw} {g₁ g₂ : Game pw}
-(h₁ : playAMoveAt g₁ |>.act) (h₂ : playAMoveAt g₂ |>.act) :
-(playAMoveAt g₁).s = (playAMoveAt g₂).s ↔ applyAMove g₁.s (g₁.a.f g₁.s
-(act_of_act_playAMoveAt h₁) (aHasValidMove_of_act_playAMoveAt h₁)).m =
-applyAMove g₂.s (g₂.a.f g₂.s (act_of_act_playAMoveAt h₂)
-(aHasValidMove_of_act_playAMoveAt h₂)).m := by
-  have H₁ := act_of_act_playAMoveAt h₁
-  have H₂ := act_of_act_playAMoveAt h₂
-  have H₃ := aHasValidMove_of_act_playAMoveAt h₁
-  have H₄ := aHasValidMove_of_act_playAMoveAt h₂
-  simp [playAMoveAt]; rw [dif_pos ⟨H₁, H₃⟩, dif_pos ⟨H₂, H₄⟩]; simp
-
-@[simp]
-theorem Game.act_playAMoveAt' {pw} {g : Game pw} {a : A pw} {h₁ h₂} :
-(playAMoveAt' a g h₁ h₂).act ↔ g.act := by rfl
-
-theorem State.finish_eq_of_not_act {s : State} (h : ¬s.act) : s.finish = s := by
-  ext:1 <;> simp_all
-
-theorem Game.finish_eq_of_not_act {pw} {g : Game pw} (h : ¬g.act) : g.finish = g := by
-  ext:1 <;> simp; exact State.finish_eq_of_not_act h
-
-@[simp]
-theorem dState_state₀ {pw} : DState pw state₀ := by
-  simp [dState_iff, State.wf_iff]; use default, default, 0; simp
-
-@[simp]
-theorem AState.aTurn {pw : outParam ℕ} {s} [hs : AState pw s] : s.aTurn = true := hs.ht
-
-@[simp]
-theorem DState.aTurn {pw : outParam ℕ} {s} [hs : DState pw s] : s.aTurn = false := hs.ht
-
-@[simp, instance]
-theorem wf_playAMoveAt {pw} {g : Game pw}
-[hs : AState pw g.s] : (playAMoveAt g).s.WF pw := by
-  rw [aState_iff] at hs; choose hs ht using hs
-  by_cases h : ¬g.s.act
-  · rw [Game.playAMoveAt_eq_of_neg # by tauto]
-    simpa [State.finish_eq_of_not_act h]
-  push Not at h
-  rw [State.wf_iff] at hs ⊢
-  choose a d n g₁ h₁ h₂ using hs
-  rcases h₂ with h₂ | ⟨h', h₂⟩
-  · have h₀ : g₁.act; simpa [Game.act, h₂]
-    contrapose h₂; clear h₂
-    apply ne_of_congr (·.aTurn)
-    simp [ht]
-    rw [←h₁]
-    rw [Game.aTurn_play_eq_of_act]; simp
-    simpa [h₁]
-  generalize hg₀ : (initGame (a.set g.s g.a) d state₀).play n = g₀
-  generalize hg' : (initGame (a.set g.s g.a) d state₀).play (n + 1) = g'
-  refine' ⟨_, d, n + 1, g', hg', _⟩; left
-  have h₄ : g₀.s = g₁.s
-  · rw [←hg₀, ←h₁]
-    apply Game.s_play_initGame_a_set_eq_of_ne
-    intro k hk H₁
-    apply ne_of_congr (·.history.length)
-    simp [←h₂, ←h₁]
-    rw [Game.length_history_play_eq_of_act H₁]
-    rw [Game.length_history_play_eq_of_act # by rwa [h₁]]
-    simp; omega
-  simp [hg₀] at hg'
-  have h₀ : g₀.act; simpa [Game.act, h₄]
-  generalize hgx : playAMoveAt g = gx
-  generalize hgy : playDMoveAt g₀ h₀ = gy
-  replace hg' : playAMoveAt gy = g'
-  · rw [←hg']; simp [Game.playMove, h₀, hgy]
-  have Hd₀ : g₀.d = d; simp [←hg₀]
-  have Hd₁ : g₁.d = d; simp [←h₁]
-  have H₁ : gy.s = g.s
-  · simp [←hgy, ←h₂, Hd₀, Hd₁]; rw! [h₄]; rfl
-  have H₂ : gy.act; simp [←hgy]
-  by_cases H₃ : ¬AHasValidMove pw g.s.board
-  · rw [←hg', Game.playAMoveAt_eq_of_neg # by grind]
-    rw [←hgx, Game.playAMoveAt_eq_of_neg # by grind]
-    simp [H₁]
-  push Not at H₃
-  have H₄ : g'.act
-  · simp [←hg']
-    rw [Game.playAMoveAt_eq_of_pos H₂ # by grind]
-    simpa [playAMoveAt']
-  have H₅ : gx.act
-  · rw [←hgx]; rwa [Game.playAMoveAt_eq_of_pos h H₃]
-  simp [←hg', ←hgx]
-  rw [Game.s_playAMoveAt_eq_iff_of_act_playAMoveAt (by grind) (by grind)]
-  rw! [H₁]; congr 2; simp [←hgy, ←hg₀, A.set]
-
-@[simp, instance]
-theorem Game.wf_playMove {pw} {g : Game pw}
-[hs : DState pw g.s] : g.playMove.s.WF pw := by
-  simp [playMove]; split_ifs <;> infer_instance
-
-theorem Game.playAMoveAt_eq_of_act {pw} {g : Game pw}
-(h : (playAMoveAt g).act) : playAMoveAt g = playAMoveAt' g.a g
-(act_of_act_playAMoveAt h) (aHasValidMove_of_act_playAMoveAt h) := by
-  simp [playAMoveAt, act_of_act_playAMoveAt h, aHasValidMove_of_act_playAMoveAt h]
-
-theorem Game.aTurn_playAMoveAt_of_act {pw} {g : Game pw}
-(h : (playAMoveAt g).act) : (playAMoveAt g).s.aTurn = !g.s.aTurn := by
-  simp [playAMoveAt_eq_of_act h]
-
-theorem dState_playAMoveAt_of_act {pw} {g : Game pw} [hs : AState pw g.s]
-(h : (playAMoveAt g).s.act) : DState pw (playAMoveAt g).s := by
-  constructor; simp [Game.aTurn_playAMoveAt_of_act h]
-
-theorem Game.dState_playMove_of_act {pw} {g : Game pw}
-[hs : DState pw g.s] (h : g.playMove.act) : DState pw g.playMove.s := by
-  constructor; rw [aTurn_playMove_eq_of_act h, hs.ht]
-
-@[simp, instance]
-theorem Game.wf_play {pw} {g : Game pw} {n} [hs : DState pw g.s] : (g.play n).s.WF pw := by
-  induction n; simp; infer_instance
-  nm n ih; simp; by_cases h₁ : (g.play n).s.act
-  · suffices : DState pw (g.play n).s; infer_instance
-    constructor; rw [aTurn_play_eq_of_act h₁, hs.ht]
-  rwa [playMove_eq_of_not_act h₁]
-
-theorem Game.dState_play_of_act {pw} {g : Game pw} {n}
-[hs : DState pw g.s] (h : (g.play n).act) : DState pw (g.play n).s := by
-  constructor; rw [aTurn_play_eq_of_act h, hs.ht]
-
-theorem not_dHws_of_aHws {pw} (h : AHws pw) : ¬DHws pw := by
-  obtain ⟨a, h⟩ := h; simp [DHws, DHwsAt]
-  intro d; use a; specialize h d; exact h
-
-theorem not_aHws_of_dHws {pw} (h : DHws pw) : ¬AHws pw := by
-  contrapose! h; exact not_dHws_of_aHws h
-
-@[simp, instance]
-theorem State.wf_toAltH_state₀ {pw} : sys.WF # state₀.toAltH pw := by
-  simp
-
-@[simp, instance]
-theorem State.wf_getd_toAltH?_state₀ {pw} : sys.WF # state₀.toAltH? pw |>.getd :=
-  wf_toAltH_state₀
-
-@[simp]
-theorem State.even_length_history_of_dState {pw s} [hs : DState pw s] :
-Even s.history.length := by
-  have h := hs.ht; simp [aTurn] at h; exact h
-
-@[simp]
-theorem State.not_odd_length_history_of_dState {pw s} [hs : DState pw s] :
-¬Odd s.history.length := by simp
-
-@[simp]
-theorem State.aTurn_eq_of_DState {pw s} [hs : DState pw s] : s.aTurn = false := by
-  simp [aTurn]
-
-theorem Board.getd_toAltH?_eq_toAlt_of {pw t₁ t₂} {b₁ b₂ : Board}
-(h : ∃ s₁ s₂, sys.WF s₁ ∧ sys.WF s₂ ∧ b₁.toAlt pw t₁ s₁.hist = s₁ ∧
-b₂.toAlt pw t₂ s₂.hist = s₂ ∧ s₁ = s₂.setHist s₁.hist) :
-∃ hist, (b₁.toAltH? pw t₁).getd = b₂.toAlt pw t₂ hist := by
-  choose s₁ s₂ hs₁ hs₂ h₁ h₂ h₃ using h
-  have h₄ : ∃ s, sys.WF s ∧ b₁.toAlt pw t₁ s.hist = s; tauto
-  have h₅ := Classical.epsilon_spec h₄
-  generalize h₆ : (Classical.epsilon _ : AP.State) = s at h₅
-  choose hs h₅ using h₅; use s.hist
-  rw [toAltH?, choose?_eq_of_pos h₄, h₆]
-  clear h₆; simp; rw [←h₅]
-  generalize s₁.hist = ps₁ at *
-  generalize s₂.hist = ps₂ at *
-  generalize s.hist = ps at *
-  subst h₂ h₃ h₅
-  simp [AP.State.ext_iff] at h₁ ⊢
-  rcases h₁ with ⟨H₁, H₂, rfl⟩
-  simp [H₁, H₂]
-
--- theorem Game.toAltH_playDMoveAt {pw} {g : Game pw} {h} [hs : DState pw g.s] :
--- ∃ hist s', (g.s.toAltH pw).dMove (Point.toAlt # g.d.f g.s h) = some s' ∧
--- (playDMoveAt g h).s.toAltH pw = s'.setHist hist
--- 
--- #check 0 #exit
-
--- @[simp, instance]
--- theorem State.wf_toAltH {pw} {s : State} [hs : s.WF pw] : sys.WF # s.toAltH pw := by
---   rw [wf_iff] at hs
---   choose a d n g h₁ h₂ using hs
---   induction n generalizing g
---   ·
---     simp at h₁
---     simp [←h₁] at h₂
---     rcases h₂ with rfl | ⟨h', h₂⟩; simp
-
--- @[simp]
--- theorem State.pw_toAltH {pw} {s : State} : (s.toAltH pw).pw = pw := by
---   unfold toAltH toAltH? Board.toAltH?
-
-theorem Board.toAlt_eq_setHist {s : State} {pw t hist} (hist₁ : List PointZ) :
-s.board.toAlt pw t hist = (s.board.toAlt pw t hist₁).setHist hist := rfl
-
-theorem Board.toAlt_eq_setHist_nil {s : State} {pw t hist} :
-s.board.toAlt pw t hist = (s.board.toAlt pw t []).setHist hist := rfl
-
-theorem State.exi_wf_toAlt_board_iff_exi_hist {pw t} {s : State} :
-(∃ s₁, sys.WF s₁ ∧ s.board.toAlt pw t s₁.hist = s₁) ↔
-∃ hist, sys.WF (s.board.toAlt pw t hist) := by
-  constructor
-  · rintro ⟨s₁, hs₁, h₁⟩; use s₁.hist; rwa [h₁]
-  · rintro ⟨hist, h⟩; use s.board.toAlt pw t hist, h; simp
-
-theorem State.exi_hist_toAlt_board_of_wfCnd {pw t} {s : State}
-(h : WFCnd # s.board.toAlt pw t []) : ∃ hist, sys.WF # s.board.toAlt pw t hist := by
-  conv => right; ext; rw [Board.toAlt_eq_setHist_nil]
-  exact AP.State.exi_hist_wf_of_wfCnd h
-
-theorem State.exi_wf_toAlt_board_of_wfCnd {pw t} {s : State}
-(h : WFCnd # s.board.toAlt pw t []) :
-∃ s₁, sys.WF s₁ ∧ s.board.toAlt pw t s₁.hist = s₁ := by
-  rw [exi_wf_toAlt_board_iff_exi_hist]; exact exi_hist_toAlt_board_of_wfCnd h
-
-@[simp]
-theorem Game.squares_board_playAMoveAt {pw} {g : Game pw} :
-(playAMoveAt g).s.board.squares = g.s.board.squares := by
-  rw [playAMoveAt]; split_ifs <;> rfl
-
-theorem State.finite_univ_diff_squares_of_play' {pw} {a : A pw} {d n g s}
-(h₁ : (Set.univ \ s.board.squares).Finite) (h₂ : (initGame a d s).play n = g) :
-(Set.univ \ g.s.board.squares).Finite := by
-  induction n generalizing s
-  · simp at h₂; simpa [←h₂]
-  nm n ih
-  rw [Game.play_succ'] at h₂
-  generalize hg₀ : (initGame a d s).playMove = g₀ at h₂
-  apply @ih g₀.s
-  rotate_left
-  · convert h₂
-    subst hg₀
-    ext :1 <;> simp
-  subst hg₀
-  simp [Game.playMove]
-  split_ifs with h₃; on_goal 2 => simpa
-  simp [playDMoveAt, applyDMove, applyDMoveB]
-  split; assumption; simpa
-
-@[simp]
-theorem State.finite_univ_diff_squares_of_play {pw} {a : A pw} {d n g}
-(h : (initGame a d state₀).play n = g) : (Set.univ \ g.s.board.squares).Finite := by
-  apply finite_univ_diff_squares_of_play' _ h; simp
-
-@[simp]
-theorem State.finite_univ_diff_squares {s pw} [hs : WF pw s] :
-.univ \ s.board.squares |>.Finite := by
-  rw [wf_iff] at hs; obtain ⟨a, d, n, g, h₁, h₂⟩ := hs
-  have h₃ := finite_univ_diff_squares_of_play h₁
-  rcases h₂ with rfl | ⟨h₂, rfl⟩; exact h₃
-  simp [playDMoveAt, applyDMove, applyDMoveB]
-  split; exact h₃; simpa
-
-@[simp]
-theorem State.finite_image_univ_diff_squares {s pw} [hs : WF pw s] :
-(·.toAlt) '' (.univ \ s.board.squares) |>.Finite := by
-  apply Set.Finite.image; simp
-
-@[simp]
-theorem State.mem_ofSet_image_univ_diff_squares {s pw p} [hs : WF pw s] :
-p ∈ Set'.ofSet ((·.toAlt) '' (.univ \ s.board.squares)) ↔
-p ∈ (·.toAlt) '' (.univ \ s.board.squares) := by
-  simp [Set'.mem_ofSet]
-
-@[simp]
-theorem Point.toAlt_eq_iff {a b : Point} : a.toAlt = b.toAlt ↔ a = b := by
-  symm; constructor; rintro rfl; rfl
-  intro h; simp [toAlt] at h; ext <;> tauto
-
--- #check 0 #exit
-
--- theorem State.exi_toAlt_board_not_aTurn_of_dState {pw s} [hs : DState pw s] :
--- ∃ s₁, sys.WF s₁ ∧ s.board.toAlt pw false s₁.hist = s₁ := by
---   cases hs; nm hs ht
---   apply exi_wf_toAlt_board_of_wfCnd
---   constructor
---   ·
---     simp
---     sorry
---   ·
---     sorry
---   ·
---     sorry
---   ·
---     sorry
-
--- #check 0 #exit
--- 
--- theorem State.exi_toAlt_board_of_dState {pw s t} [hs : DState pw s] :
--- ∃ s₁, sys.WF s₁ ∧ s.board.toAlt pw t s₁.hist = s₁ := by
--- 
--- #check 0 #exit
--- 
--- theorem Game.toAltH_playDMoveAt_of_none {pw} {g : Game pw} {h} [hs : DState pw g.s]
--- (h₁ : (g.d.f g.s h).m = none) : ∃ hist,
--- (playDMoveAt g h).s.toAltH pw = g.s.toAlt pw hist := by
---   simp [playDMoveAt, applyDMove, applyDMoveB, h₁, applyMove,State.toAltH,
---     State.toAltH?, State.toAlt]
---   
---   congr 1
---   apply Board.getd_toAltH?_eq_toAlt_of
---   simp_rw [State.toAlt_eq]
--- 
--- #check 0 #exit
--- 
--- theorem dHws_and_dwn_lt_toAltH_playDMoveAt_dOptimal_of_dHws {pw} {g g₁ : Game pw} {h}
--- [hs : DState pw g.s]
--- (h₁ : g.d = (dOptimal pw).getd)
--- (h₂ : g.s.toAltH pw |>.dHws)
--- (hg₁ : playDMoveAt g h = g₁) :
--- (g₁.s.toAltH pw).dHws ∧ g₁.s.dwn pw < g.s.dwn pw := by
---   split_ands
---   ·
---     simp [←hg₁]
--- 
--- #check 0 #exit
--- 
--- theorem DHws_of_alt {pw} (h : AP.dHwsPw pw) : DHws pw := by
---   specialize h 0
---   generalize h₀ : state₀ = s
---   
---   replace h : s.toAltH pw |>.dHws
---   ·
---     subst h₀
---     simp [State.toAltH, State.toAltH?, Board.toAltH?]
---     
---     apply choose?_of_pos (P := λ (x : Option AP.State) => x.getd.dHws) _ _
---     ·
---       use AP.initState pw 0
---       simp
---     
---     rintro s - ⟨hs, h₂⟩
---     simp at h₂ ⊢
---     rw [setHist_eq_comm] at h₂
---     simp at h₂
---     rw [←h₂] at h
---     
---     have h₁ : sys.WF # s.setHist [0]
---     ·
---       simp [h₂]
---     
---     simp at h
---     exact h
---   
---   have h₁ : s.toAltH pw = AP.initState pw 0
---   ·
---     simp [←h₀]
---   
---   generalize hn : s.dwn pw = n
---   generalize h₂ : (dOptimal pw).getd = d
---   use d
---   intro a
---   have hs : sys.WF # s.toAltH pw; simp [h₁]
---   
---   rw [h₀]
---   have h₃ : s.act
---   ·
---     rw [←h₀]
---     simp
---   
---   have ht : s.aTurn = false
---   ·
---     simp [←h₀]
---   
---   clear h₀ h₁
---   
---   use n
---   
---   induction n using Nat.strong_induction_on generalizing s
+-- theorem Game.act_play_initGame_of_not_aTurn {pw a d n g s}
+-- (h₁ : s.aTurn = false) (h₂ : s.act) (h₃ : (initGame a d s : Game pw).play n = g)
+-- (h₄ : g.s.aTurn = false) : g.s.act := by
+--   induction n generalizing s g
+--   · simp at h₃; simpa [←h₃]
 --   nm n ih
---   cases n
---   ·
---     contrapose! hn
---     simpa [State.dwn_eq, State.dwn_eq_zero_iff_aHws]
---   nm n
---   simp at ih
---   
---   rw [Game.play_succ', Game.playMove]
---   simp [h₃, playAMoveAt]
---   rw! [eq_true_of Game.act_playDMoveAt]
---   rw! (castMode := .all) [true_and]
---   
---   split_ifs with h₄
---   on_goal 2 => simp
---   
---   generalize_proofs H₁ H₂ H₃
---   by_contra H
---   generalize hg₁ : playDMoveAt (initGame a d s) H₁ = g₁
---   contrapose H; clear H
---   rw! [hg₁] at h₄ ⊢
---   
---   have ht₁ : g₁.s.aTurn = true
---   ·
---     clear ih
---     subst hg₁
+--   rw [play_succ'] at h₃
+--   simp [playMove, h₂] at h₃
+--   simp [playDMoveAt] at h₃
+--   generalize_proofs at h₃
+--   generalize h₅ : applyDMove s (d.f s h₂).m = s₁ at h₃
+--   have h₆ : s₁.act; simpa [←h₅]
+--   simp [playAMoveAt] at h₃
+--   split_ifs at h₃ with h₇
+--   rotate_left
+--   · replace h₃ := congrArg (·.s.aTurn) h₃
+--     simp [←h₅, h₁, h₄] at h₃
+--   simp [playAMoveAt'] at h₃
+--   generalize_proofs at h₃
+--   generalize hs₂ : applyAMove s₁ (a.f s₁ h₆ h₇).m = s₂ at h₃
+--   have H₁ : s₂.act; simpa [←hs₂]
+--   have H₂ : s₁.aTurn = true; simpa [←h₅]
+--   have H₃ : s₂.aTurn = false; simpa [←hs₂]
+--   grind
+-- 
+-- @[simp]
+-- theorem Game.s_playAMoveAt'_eq_iff {pw} {g₁ g₂ : Game pw} {h₁ h₂ h₃ h₄} :
+-- (playAMoveAt' g₁.a g₁ h₁ h₂).s = (playAMoveAt' g₂.a g₂ h₃ h₄).s ↔
+-- applyAMove g₁.s (g₁.a.f g₁.s h₁ h₂).m = applyAMove g₂.s (g₂.a.f g₂.s h₃ h₄).m := by rfl
+-- 
+-- @[simp]
+-- theorem Game.s_playDMoveAt_eq_iff {pw} {g₁ g₂ : Game pw} {h₁ h₂} :
+-- (playDMoveAt g₁ h₁).s = (playDMoveAt g₂ h₂).s ↔
+-- applyDMove g₁.s (g₁.d.f g₁.s h₁).m = applyDMove g₂.s (g₂.d.f g₂.s h₂).m := by rfl
+-- 
+-- @[simp] theorem Game.a_finish {pw} {g : Game pw} : g.finish.a = g.a := rfl
+-- @[simp] theorem Game.d_finish {pw} {g : Game pw} : g.finish.d = g.d := rfl
+-- 
+-- @[simp] theorem Game.a_setState {pw} {g : Game pw} {s} : (g.setState s).a = g.a := rfl
+-- @[simp] theorem Game.d_setState {pw} {g : Game pw} {s} : (g.setState s).d = g.d := rfl
+-- 
+-- @[simp]
+-- theorem Game.a_playAMoveAt' {pw} {g : Game pw} {a : A pw} {h₁ h₂} :
+-- (playAMoveAt' a g h₁ h₂).a = g.a := rfl
+-- 
+-- @[simp]
+-- theorem Game.d_playAMoveAt' {pw} {g : Game pw} {a : A pw} {h₁ h₂} :
+-- (playAMoveAt' a g h₁ h₂).d = g.d := rfl
+-- 
+-- @[simp]
+-- theorem Game.a_playAMoveAt {pw} {g : Game pw} : (playAMoveAt g).a = g.a := by
+--   simp [playAMoveAt]; split_ifs <;> simp
+-- 
+-- @[simp]
+-- theorem Game.d_playAMoveAt {pw} {g : Game pw} : (playAMoveAt g).d = g.d := by
+--   simp [playAMoveAt]; split_ifs <;> simp
+-- 
+-- @[simp]
+-- theorem Game.a_playDMoveAt {pw} {g : Game pw} {h} : (playDMoveAt g h).a = g.a := by
+--   simp [playDMoveAt]
+-- 
+-- @[simp]
+-- theorem Game.d_playDMoveAt {pw} {g : Game pw} {h} : (playDMoveAt g h).d = g.d := by
+--   simp [playDMoveAt]
+-- 
+-- @[simp]
+-- theorem Game.a_playMove {pw} {g : Game pw} : g.playMove.a = g.a := by
+--   simp [playMove]; split_ifs <;> simp
+-- 
+-- @[simp]
+-- theorem Game.d_playMove {pw} {g : Game pw} : g.playMove.d = g.d := by
+--   simp [playMove]; split_ifs <;> simp
+-- 
+-- @[simp]
+-- theorem Game.a_play {pw} {g : Game pw} {n} : (g.play n).a = g.a := by
+--   induction n; rfl; simpa [play_succ]
+-- 
+-- @[simp]
+-- theorem Game.d_play {pw} {g : Game pw} {n} : (g.play n).d = g.d := by
+--   induction n; rfl; simpa [play_succ]
+-- 
+-- @[simp]
+-- theorem State.board_finish {s : State} : s.finish.board = s.board := rfl
+-- 
+-- theorem Game.s_playAMoveAt_eq_iff_of {pw} {g₁ g₂ : Game pw} (h₁ : g₁.s.act ↔ g₂.s.act)
+-- (h₂ : AHasValidMove pw g₁.s.board ↔ AHasValidMove pw g₂.s.board) : ∀ h₁ h₂ h₃ h₄,
+-- (playAMoveAt g₁).s = (playAMoveAt g₂).s ↔
+-- applyAMove g₁.s (g₁.a.f g₁.s h₁ h₂).m = applyAMove g₂.s (g₂.a.f g₂.s h₃ h₄).m := by
+--   simp_all [playAMoveAt, playAMoveAt', applyAMove, act]
+-- 
+-- theorem Game.playAMoveAt_eq_of_neg {pw} {g : Game pw}
+-- (h : ¬g.s.act ∨ ¬AHasValidMove pw g.s.board) : playAMoveAt g = g.finish := by
+--   simp [playAMoveAt]; tauto
+-- 
+-- theorem Game.s_play_initGame_d_set_eq_of_ne {pw a d s s₁ dRef n}
+-- (h : ∀ k < n, (initGame a d s |>.play k : Game pw).s ≠ s₁) :
+-- (initGame a (d.set s₁ dRef) s |>.play n).s = (initGame a d s |>.play n).s := by
+--   induction n; simp
+--   nm n ih
+--   specialize ih # by grind
+--   simp [play_succ, playMove, act]
+--   rw! (castMode := .all) [ih]
+--   split_ifs with h₁
+--   on_goal 2 => exact ih
+--   generalize hg : (initGame a d s).play n = g at *
+--   generalize hg₁ : (initGame a (d.set s₁ dRef) s).play n = g₁ at *
+--   have H₁ : g₁.a = g.a; simp [←hg, ←hg₁]
+--   simp [playDMoveAt]
+--   rw! [ih]
+--   have h₂ : applyDMove g.s (g₁.d.f g.s h₁).m = applyDMove g.s (g.d.f g.s h₁).m
+--   · congr 2; simp [←hg₁, D.set]
+--     rw [if_neg]; simp [←hg]
+--     rw [←hg]; apply h; omega
+--   rw [h₂]
+--   generalize h₃ : applyDMove g.s (g.d.f g.s h₁).m = s'
+--   have h₄ : s'.act; simpa [←h₃]
+--   by_cases h₅ : ¬AHasValidMove pw s'.board
+--   · iterate 2 rw [playAMoveAt_eq_of_neg # by tauto];; simp
+--   push Not at h₅
+--   have h₆ := @s_playAMoveAt_eq_iff_of _ (g₁.setState s') (g.setState s')
+--     (by simp) (by simp) (by simpa) (by simpa) (by simpa) (by simpa)
+--   rw [h₆]; clear h₆
+--   simp; grind
+-- 
+-- theorem Game.act_of_act_playMove {pw} {g : Game pw} (h : g.playMove.s.act) : g.s.act := by
+--   by_contra h₁; simp [playMove_eq, h₁] at h
+-- 
+-- theorem Game.act_of_act_play {pw} {g : Game pw} {n} (h : (g.play n).s.act) : g.s.act := by
+--   induction n; simp at h; exact h
+--   nm n ih; apply ih
+--   simp [play_succ] at h
+--   exact act_of_act_playMove h
+-- 
+-- @[simp]
+-- theorem State.length_history_applyAMove {s m} :
+-- (applyAMove s m).history.length = s.history.length + 1 := by
+--   simp [applyAMove]
+-- 
+-- @[simp]
+-- theorem State.length_history_applyDMove {s m} :
+-- (applyDMove s m).history.length = s.history.length + 1 := by
+--   simp [applyDMove]
+-- 
+-- @[simp]
+-- theorem Game.length_history_playAMoveAt' {pw} {g : Game pw} {a : A pw} {h₁ h₂} :
+-- (playAMoveAt' a g h₁ h₂).s.history.length = g.s.history.length + 1 := by
+--   simp [playAMoveAt']
+-- 
+-- @[simp]
+-- theorem Game.length_history_playDMoveAt {pw} {g : Game pw} {h} :
+-- (playDMoveAt g h).s.history.length = g.s.history.length + 1 := by
+--   simp [playDMoveAt]
+-- 
+-- @[simp]
+-- theorem State.history_finish {s : State} : s.finish.history = s.history := rfl
+-- 
+-- theorem Game.length_history_playMove_eq_of_act {pw} {g : Game pw}
+-- (h : g.playMove.s.act) : g.playMove.s.history.length = g.s.history.length + 2 := by
+--   have h₁ := act_of_act_playMove h
+--   simp [h₁, playMove, playAMoveAt]
+--   rw [dif_pos]; simp
+--   simp [playMove, h₁, playAMoveAt] at h
+--   split_ifs at h with h₂ <;> simp_all
+-- 
+-- theorem Game.length_history_play_eq_of_act {pw} {g : Game pw} {n}
+-- (h : (g.play n).act) : (g.play n).s.history.length = g.s.history.length + n * 2 := by
+--   induction n; simp; nm n ih
+--   simp [play_succ] at h ⊢
+--   specialize ih # act_of_act_playMove h
+--   rw [length_history_playMove_eq_of_act h]; omega
+-- 
+-- @[simp]
+-- theorem Game.play_add {pw} {g : Game pw} {n m} : g.play (n + m) = (g.play n).play m := by
+--   nth_rw 1 [play, add_comm]; rw [Function.iterate_add]; rfl
+-- 
+-- theorem Game.s_play_eq_iff_of_act {pw} {g : Game pw} {n m}
+-- (h : g.play (max n m) |>.act) : (g.play n).s = (g.play m).s ↔ n = m := by
+--   symm; constructor; rintro rfl; rfl
+--   contrapose!
+--   intro h₁
+--   apply ne_of_congr (·.history.length)
+--   wlog h₂ : n < m with ih; grind
+--   clear h₁
+--   rw [max_eq_right_of_lt h₂] at h
+--   obtain ⟨m, rfl⟩ := Nat.exists_eq_add_of_le # le_of_lt h₂
+--   simp at h ⊢
+--   rw [length_history_play_eq_of_act h]; omega
+-- 
+-- @[simp]
+-- theorem history_state₀ : state₀.history = [] := rfl
+-- 
+-- @[simp]
+-- theorem Game.aTurn_playAMoveAt' {pw} {g : Game pw} {a : A pw} {h₁ h₂} :
+-- (playAMoveAt' a g h₁ h₂).s.aTurn = !g.s.aTurn := by
+--   simp [playAMoveAt']
+-- 
+-- theorem Game.aTurn_playMove_eq_of_act {pw} {g : Game pw}
+-- (h : g.playMove.s.act) : g.playMove.s.aTurn = g.s.aTurn := by
+--   simp [playMove] at h ⊢
+--   split_ifs at h ⊢ with h₁; on_goal 2 => contradiction
+--   generalize hg₁ : playDMoveAt g h₁ = g₁ at h ⊢
+--   have h₂ : g₁.s.act; simpa [←hg₁]
+--   simp [playAMoveAt] at h ⊢
+--   rw! (castMode := .all) [Game.act, eq_true_of h₂, true_and] at h ⊢
+--   split_ifs at h ⊢ with h₃; on_goal 2 => simp at h
+--   simp [←hg₁]
+-- 
+-- theorem Game.aTurn_play_eq_of_act {pw} {g : Game pw} {n}
+-- (h : (g.play n).act) : (g.play n).s.aTurn = g.s.aTurn := by
+--   induction n; simp; nm n ih; simp at h ⊢
+--   specialize ih (act_of_act_playMove h)
+--   rwa [aTurn_playMove_eq_of_act h]
+-- 
+-- theorem aState_iff {pw s} : AState pw s ↔ s.WF pw ∧ s.aTurn = true := by
+--   constructor <;> rintro ⟨⟩ <;> constructor <;> assumption
+-- 
+-- theorem dState_iff {pw s} : DState pw s ↔ s.WF pw ∧ s.aTurn = false := by
+--   constructor <;> rintro ⟨⟩ <;> constructor <;> assumption
+-- 
+-- @[simp, instance]
+-- theorem aState_playDMoveAt {pw} {g : Game pw} {h}
+-- [hs : DState pw g.s] : AState pw (playDMoveAt g h).s := by
+--   rw [dState_iff] at hs; choose hs ht using hs; rw [aState_iff]
+--   rw [State.wf_iff] at hs ⊢
+--   symm; split_ands; simpa
+--   choose a d n g₁ h₁ h₂ using hs
+--   symm at h₂; rcases h₂ with ⟨h', h₂⟩ | h₂
+--   · contrapose h₂; clear h₂
+--     apply ne_of_congr (·.aTurn)
+--     simp [ht]
+--     rw [←h₁] at h' ⊢
+--     simp [Game.aTurn_play_eq_of_act h']
+--   have h₃ : g₁.s.act
+--   · replace h₂ := congrArg (·.aTurn) h₂
+--     simp [ht] at h₂
+--     apply Game.act_play_initGame_of_not_aTurn _ _ h₁ <;> simp_all
+--   generalize hg' : (initGame a (d.set g₁.s g.d) state₀).play n = g'
+--   refine' ⟨a, _, n, g', hg', _⟩; right
+--   have h₄ : g'.s = g.s
+--   · rw [←h₂, ←h₁, ←hg']
+--     apply Game.s_play_initGame_d_set_eq_of_ne
+--     intro k hk
+--     simp [←h₁]
+--     rw [Game.s_play_eq_iff_of_act]; omega
+--     rw [max_eq_right_of_lt hk, h₁]
+--     exact h₃
+--   simp [h₄, h, applyDMove, applyMove]
+--   congr 1; simp [←hg', D.set]; grind
+-- 
+-- theorem Game.playAMoveAt_eq_of_not_act {pw} {g : Game pw}
+-- (h : ¬g.s.act) : playAMoveAt g = g.finish := by
+--   simp [playAMoveAt, h]
+-- 
+-- theorem Game.s_play_initGame_a_set_eq_of_ne {pw a d s s₁ aRef n}
+-- (h : ∀ k < n, ∀ h, (playDMoveAt (initGame a d s |>.play k) h : Game pw).s ≠ s₁) :
+-- (initGame (a.set s₁ aRef) d s |>.play n).s = (initGame a d s |>.play n).s := by
+--   induction n; simp
+--   nm n ih
+--   specialize ih # by grind
+--   simp [play_succ, playMove, act]
+--   rw! (castMode := .all) [ih]
+--   split_ifs with h₁
+--   on_goal 2 => exact ih
+--   generalize hg : (initGame a d s).play n = g at *
+--   generalize hg₁ : (initGame (a.set s₁ aRef) d s).play n = g₁ at *
+--   generalize_proofs H₁
+--   generalize hgx : playDMoveAt g₁ H₁ = gx
+--   generalize hgy : playDMoveAt g h₁ = gy
+--   have H₂ : gx.s = gy.s
+--   · subst hgx hgy
+--     simp
+--     congr 1
+--     simp [←hg₁, ←hg]
+--     rw! [ih]
+--     rfl
+--   simp [playAMoveAt, act]
+--   rw! (castMode := .all) [H₂]
+--   split_ifs with H₃; on_goal 2 => simp [H₂]
+--   rcases H₃ with ⟨H₃, H₄⟩
+--   simp
+--   have H₅ : gx.a = a.set s₁ aRef; simp [←hgx, ←hg₁]
+--   have H₆ : gy.a = a; simp [←hgy, ←hg]
+--   rw! [H₅, H₆, ←H₂]
+--   congr 2
+--   simp [A.set]
+--   contrapose!; rintro - rfl
+--   contrapose h; clear h
+--   simp
+--   use n, by rfl
+--   simp [hg, h₁, hgy, H₂]
+-- 
+-- theorem Game.playAMoveAt_eq_of_pos {pw} {g : Game pw}
+-- (h₁ : g.s.act) (h₂ : AHasValidMove pw g.s.board) :
+-- playAMoveAt g = playAMoveAt' g.a g h₁ h₂ := by
+--   simp [playAMoveAt, h₁, h₂]
+-- 
+-- theorem Game.act_of_act_playAMoveAt {pw} {g : Game pw} (h : playAMoveAt g |>.act) : g.s.act := by
+--   by_contra! h₁; simp [playAMoveAt, h₁] at h
+-- 
+-- theorem Game.aHasValidMove_of_act_playAMoveAt {pw} {g : Game pw}
+-- (h : playAMoveAt g |>.act) : AHasValidMove pw g.s.board := by
+--   by_contra! h₁; simp [playAMoveAt, h₁] at h
+-- 
+-- theorem Game.s_playAMoveAt_eq_iff_of_act_playAMoveAt {pw} {g₁ g₂ : Game pw}
+-- (h₁ : playAMoveAt g₁ |>.act) (h₂ : playAMoveAt g₂ |>.act) :
+-- (playAMoveAt g₁).s = (playAMoveAt g₂).s ↔ applyAMove g₁.s (g₁.a.f g₁.s
+-- (act_of_act_playAMoveAt h₁) (aHasValidMove_of_act_playAMoveAt h₁)).m =
+-- applyAMove g₂.s (g₂.a.f g₂.s (act_of_act_playAMoveAt h₂)
+-- (aHasValidMove_of_act_playAMoveAt h₂)).m := by
+--   have H₁ := act_of_act_playAMoveAt h₁
+--   have H₂ := act_of_act_playAMoveAt h₂
+--   have H₃ := aHasValidMove_of_act_playAMoveAt h₁
+--   have H₄ := aHasValidMove_of_act_playAMoveAt h₂
+--   simp [playAMoveAt]; rw [dif_pos ⟨H₁, H₃⟩, dif_pos ⟨H₂, H₄⟩]; simp
+-- 
+-- @[simp]
+-- theorem Game.act_playAMoveAt' {pw} {g : Game pw} {a : A pw} {h₁ h₂} :
+-- (playAMoveAt' a g h₁ h₂).act ↔ g.s.act := by rfl
+-- 
+-- theorem State.finish_eq_of_not_act {s : State} (h : ¬s.act) : s.finish = s := by
+--   ext:1 <;> simp_all
+-- 
+-- theorem Game.finish_eq_of_not_act {pw} {g : Game pw} (h : ¬g.s.act) : g.finish = g := by
+--   ext:1 <;> simp; exact State.finish_eq_of_not_act h
+-- 
+-- @[simp]
+-- theorem dState_state₀ {pw} : DState pw state₀ := by
+--   simp [dState_iff, State.wf_iff]; use default, default, 0; simp
+-- 
+-- @[simp]
+-- theorem AState.aTurn {pw : outParam ℕ} {s} [hs : AState pw s] : s.aTurn = true := hs.ht
+-- 
+-- @[simp]
+-- theorem DState.aTurn {pw : outParam ℕ} {s} [hs : DState pw s] : s.aTurn = false := hs.ht
+-- 
+-- @[simp, instance]
+-- theorem wf_playAMoveAt {pw} {g : Game pw}
+-- [hs : AState pw g.s] : (playAMoveAt g).s.WF pw := by
+--   rw [aState_iff] at hs; choose hs ht using hs
+--   by_cases h : ¬g.s.act
+--   · rw [Game.playAMoveAt_eq_of_neg # by tauto]
+--     simpa [State.finish_eq_of_not_act h]
+--   push Not at h
+--   rw [State.wf_iff] at hs ⊢
+--   choose a d n g₁ h₁ h₂ using hs
+--   rcases h₂ with h₂ | ⟨h', h₂⟩
+--   · have h₀ : g₁.s.act; simpa [h₂]
+--     contrapose h₂; clear h₂
+--     apply ne_of_congr (·.aTurn)
+--     simp [ht]
+--     rw [←h₁]
+--     rw [Game.aTurn_play_eq_of_act]; simp
+--     simpa [h₁]
+--   generalize hg₀ : (initGame (a.set g.s g.a) d state₀).play n = g₀
+--   generalize hg' : (initGame (a.set g.s g.a) d state₀).play (n + 1) = g'
+--   refine' ⟨_, d, n + 1, g', hg', _⟩; left
+--   have h₄ : g₀.s = g₁.s
+--   · rw [←hg₀, ←h₁]
+--     apply Game.s_play_initGame_a_set_eq_of_ne
+--     intro k hk H₁
+--     apply ne_of_congr (·.history.length)
+--     simp [←h₂, ←h₁]
+--     rw [Game.length_history_play_eq_of_act H₁]
+--     rw [Game.length_history_play_eq_of_act # by rwa [h₁]]
+--     simp; omega
+--   simp [hg₀] at hg'
+--   have h₀ : g₀.s.act; simpa [Game.act, h₄]
+--   generalize hgx : playAMoveAt g = gx
+--   generalize hgy : playDMoveAt g₀ h₀ = gy
+--   replace hg' : playAMoveAt gy = g'
+--   · rw [←hg']; simp [Game.playMove, h₀, hgy]
+--   have Hd₀ : g₀.d = d; simp [←hg₀]
+--   have Hd₁ : g₁.d = d; simp [←h₁]
+--   have H₁ : gy.s = g.s
+--   · simp [←hgy, ←h₂, Hd₀, Hd₁]; rw! [h₄]; rfl
+--   have H₂ : gy.s.act; simp [←hgy]
+--   by_cases H₃ : ¬AHasValidMove pw g.s.board
+--   · rw [←hg', Game.playAMoveAt_eq_of_neg # by grind]
+--     rw [←hgx, Game.playAMoveAt_eq_of_neg # by grind]
+--     simp [H₁]
+--   push Not at H₃
+--   have H₄ : g'.act
+--   · simp [←hg']
+--     rw [Game.playAMoveAt_eq_of_pos H₂ # by grind]
+--     simpa [playAMoveAt']
+--   have H₅ : gx.act
+--   · rw [←hgx]; rwa [Game.playAMoveAt_eq_of_pos h H₃]
+--   simp [←hg', ←hgx]
+--   rw [Game.s_playAMoveAt_eq_iff_of_act_playAMoveAt (by grind) (by grind)]
+--   rw! [H₁]; congr 2; simp [←hgy, ←hg₀, A.set]
+-- 
+-- @[simp, instance]
+-- theorem Game.wf_playMove {pw} {g : Game pw}
+-- [hs : DState pw g.s] : g.playMove.s.WF pw := by
+--   simp [playMove]; split_ifs <;> infer_instance
+-- 
+-- theorem Game.playAMoveAt_eq_of_act {pw} {g : Game pw}
+-- (h : (playAMoveAt g).act) : playAMoveAt g = playAMoveAt' g.a g
+-- (act_of_act_playAMoveAt h) (aHasValidMove_of_act_playAMoveAt h) := by
+--   simp [playAMoveAt, act_of_act_playAMoveAt h, aHasValidMove_of_act_playAMoveAt h]
+-- 
+-- theorem Game.aTurn_playAMoveAt_of_act {pw} {g : Game pw}
+-- (h : (playAMoveAt g).act) : (playAMoveAt g).s.aTurn = !g.s.aTurn := by
+--   simp [playAMoveAt_eq_of_act h]
+-- 
+-- theorem dState_playAMoveAt_of_act {pw} {g : Game pw} [hs : AState pw g.s]
+-- (h : (playAMoveAt g).s.act) : DState pw (playAMoveAt g).s := by
+--   constructor; simp [Game.aTurn_playAMoveAt_of_act h]
+-- 
+-- theorem Game.dState_playMove_of_act {pw} {g : Game pw}
+-- [hs : DState pw g.s] (h : g.playMove.act) : DState pw g.playMove.s := by
+--   constructor; rw [aTurn_playMove_eq_of_act h, hs.ht]
+-- 
+-- @[simp, instance]
+-- theorem Game.wf_play {pw} {g : Game pw} {n} [hs : DState pw g.s] : (g.play n).s.WF pw := by
+--   induction n; simp; infer_instance
+--   nm n ih; simp; by_cases h₁ : (g.play n).s.act
+--   · suffices : DState pw (g.play n).s; infer_instance
+--     constructor; rw [aTurn_play_eq_of_act h₁, hs.ht]
+--   rwa [playMove_eq_of_not_act h₁]
+-- 
+-- theorem Game.dState_play_of_act {pw} {g : Game pw} {n}
+-- [hs : DState pw g.s] (h : (g.play n).act) : DState pw (g.play n).s := by
+--   constructor; rw [aTurn_play_eq_of_act h, hs.ht]
+-- 
+-- theorem not_dHws_of_aHws {pw} (h : AHws pw) : ¬DHws pw := by
+--   obtain ⟨a, h⟩ := h; simp [DHws, DHwsAt]
+--   intro d; use a; specialize h d; exact h
+-- 
+-- theorem not_aHws_of_dHws {pw} (h : DHws pw) : ¬AHws pw := by
+--   contrapose! h; exact not_dHws_of_aHws h
+-- 
+-- @[simp, instance]
+-- theorem State.wf_toAltH_state₀ {pw} : sys.WF # state₀.toAltH pw := by
+--   simp
+-- 
+-- @[simp, instance]
+-- theorem State.wf_getd_toAltH?_state₀ {pw} : sys.WF # state₀.toAltH? pw |>.getd :=
+--   wf_toAltH_state₀
+-- 
+-- @[simp]
+-- theorem State.even_length_history_of_dState {pw s} [hs : DState pw s] :
+-- Even s.history.length := by
+--   have h := hs.ht; simp [aTurn] at h; exact h
+-- 
+-- @[simp]
+-- theorem State.not_odd_length_history_of_dState {pw s} [hs : DState pw s] :
+-- ¬Odd s.history.length := by simp
+-- 
+-- @[simp]
+-- theorem State.aTurn_eq_of_DState {pw s} [hs : DState pw s] : s.aTurn = false := by
+--   simp [aTurn]
+-- 
+-- theorem Board.getd_toAltH?_eq_toAlt_of {pw t₁ t₂} {b₁ b₂ : Board}
+-- (h : ∃ s₁ s₂, sys.WF s₁ ∧ sys.WF s₂ ∧ b₁.toAlt pw t₁ s₁.hist = s₁ ∧
+-- b₂.toAlt pw t₂ s₂.hist = s₂ ∧ s₁ = s₂.setHist s₁.hist) :
+-- ∃ hist, (b₁.toAltH? pw t₁).getd = b₂.toAlt pw t₂ hist := by
+--   choose s₁ s₂ hs₁ hs₂ h₁ h₂ h₃ using h
+--   have h₄ : ∃ s, sys.WF s ∧ b₁.toAlt pw t₁ s.hist = s; tauto
+--   have h₅ := Classical.epsilon_spec h₄
+--   generalize h₆ : (Classical.epsilon _ : AP.State) = s at h₅
+--   choose hs h₅ using h₅; use s.hist
+--   rw [toAltH?, choose?_eq_of_pos h₄, h₆]
+--   clear h₆; simp; rw [←h₅]
+--   generalize s₁.hist = ps₁ at *
+--   generalize s₂.hist = ps₂ at *
+--   generalize s.hist = ps at *
+--   subst h₂ h₃ h₅
+--   simp [AP.State.ext_iff] at h₁ ⊢
+--   rcases h₁ with ⟨H₁, H₂, rfl⟩
+--   simp [H₁, H₂]
+-- 
+-- theorem Board.toAlt_eq_setHist {s : State} {pw t hist} (hist₁ : List PointZ) :
+-- s.board.toAlt pw t hist = (s.board.toAlt pw t hist₁).setHist hist := rfl
+-- 
+-- theorem Board.toAlt_eq_setHist_nil {s : State} {pw t hist} :
+-- s.board.toAlt pw t hist = (s.board.toAlt pw t []).setHist hist := rfl
+-- 
+-- theorem State.exi_wf_toAlt_board_iff_exi_hist {pw t} {s : State} :
+-- (∃ s₁, sys.WF s₁ ∧ s.board.toAlt pw t s₁.hist = s₁) ↔
+-- ∃ hist, sys.WF (s.board.toAlt pw t hist) := by
+--   constructor
+--   · rintro ⟨s₁, hs₁, h₁⟩; use s₁.hist; rwa [h₁]
+--   · rintro ⟨hist, h⟩; use s.board.toAlt pw t hist, h; simp
+-- 
+-- theorem State.exi_hist_toAlt_board_of_wfCnd {pw t} {s : State}
+-- (h : WFCnd # s.board.toAlt pw t []) : ∃ hist, sys.WF # s.board.toAlt pw t hist := by
+--   conv => right; ext; rw [Board.toAlt_eq_setHist_nil]
+--   exact AP.State.exi_hist_wf_of_wfCnd h
+-- 
+-- theorem State.exi_wf_toAlt_board_of_wfCnd {pw t} {s : State}
+-- (h : WFCnd # s.board.toAlt pw t []) :
+-- ∃ s₁, sys.WF s₁ ∧ s.board.toAlt pw t s₁.hist = s₁ := by
+--   rw [exi_wf_toAlt_board_iff_exi_hist]; exact exi_hist_toAlt_board_of_wfCnd h
+-- 
+-- @[simp]
+-- theorem Game.squares_board_playAMoveAt {pw} {g : Game pw} :
+-- (playAMoveAt g).s.board.squares = g.s.board.squares := by
+--   rw [playAMoveAt]; split_ifs <;> rfl
+-- 
+-- theorem State.finite_univ_diff_squares_of_play' {pw} {a : A pw} {d n g s}
+-- (h₁ : (Set.univ \ s.board.squares).Finite) (h₂ : (initGame a d s).play n = g) :
+-- (Set.univ \ g.s.board.squares).Finite := by
+--   induction n generalizing s
+--   · simp at h₂; simpa [←h₂]
+--   nm n ih
+--   rw [Game.play_succ'] at h₂
+--   generalize hg₀ : (initGame a d s).playMove = g₀ at h₂
+--   apply @ih g₀.s
+--   rotate_left
+--   · convert h₂
+--     subst hg₀
+--     ext :1 <;> simp
+--   subst hg₀
+--   simp [Game.playMove]
+--   split_ifs with h₃; on_goal 2 => simpa
+--   simp [playDMoveAt, applyDMove, applyDMoveB]
+--   split; assumption; simpa
+-- 
+-- @[simp]
+-- theorem State.finite_univ_diff_squares_of_play {pw} {a : A pw} {d n g}
+-- (h : (initGame a d state₀).play n = g) : (Set.univ \ g.s.board.squares).Finite := by
+--   apply finite_univ_diff_squares_of_play' _ h; simp
+-- 
+-- @[simp]
+-- theorem State.finite_univ_diff_squares {s pw} [hs : WF pw s] :
+-- .univ \ s.board.squares |>.Finite := by
+--   rw [wf_iff] at hs; obtain ⟨a, d, n, g, h₁, h₂⟩ := hs
+--   have h₃ := finite_univ_diff_squares_of_play h₁
+--   rcases h₂ with rfl | ⟨h₂, rfl⟩; exact h₃
+--   simp [playDMoveAt, applyDMove, applyDMoveB]
+--   split; exact h₃; simpa
+-- 
+-- @[simp]
+-- theorem State.finite_image_univ_diff_squares {s pw} [hs : WF pw s] :
+-- (·.toAlt) '' (.univ \ s.board.squares) |>.Finite := by
+--   apply Set.Finite.image; simp
+-- 
+-- @[simp]
+-- theorem State.mem_ofSet_image_univ_diff_squares {s pw p} [hs : WF pw s] :
+-- p ∈ Set'.ofSet ((·.toAlt) '' (.univ \ s.board.squares)) ↔
+-- p ∈ (·.toAlt) '' (.univ \ s.board.squares) := by
+--   simp [Set'.mem_ofSet]
+-- 
+-- @[simp]
+-- theorem Point.toAlt_eq_iff {a b : Point} : a.toAlt = b.toAlt ↔ a = b := by
+--   symm; constructor; rintro rfl; rfl
+--   intro h; simp [toAlt] at h; ext <;> tauto
+-- 
+-- @[simp]
+-- theorem wf_state₀ {pw} : State.WF pw state₀ := by
+--   rw [State.wf_iff]; use default, default, 0; simp
+-- 
+-- theorem Game.aTurn_playMove_iff {pw} {g : Game pw} (ha : g.s.act) (ht : g.s.aTurn = false) :
+-- g.playMove.s.aTurn = haveI := Classical.propDecidable; !decide g.playMove.act := by
+--   simp [playMove, ha]; simp [playAMoveAt]; split_ifs with h₁ <;> simp_all
+-- 
+-- theorem Game.aTurn_play_iff {pw} {g : Game pw} {n} (ha : g.s.act) (ht : g.s.aTurn = false) :
+-- (g.play n).s.aTurn = haveI := Classical.propDecidable; !decide (g.play n).act := by
+--   induction n generalizing g
+--   · simpa [ht]
+--   nm n ih; simp; by_cases h₁ : (g.play n).act
+--   · rw [aTurn_playMove_iff h₁]
+--     contrapose h₁; simp at h₁
+--     simpa [ih ha ht]
+--   · rw [playMove_eq_of_not_act h₁, ih ha ht]
+--     simp [h₁, playMove_eq_of_not_act]
+-- 
+-- @[simp]
+-- theorem Game.length_history_le_playAMoveAt {pw} {g : Game pw} :
+-- g.s.history.length ≤ (playAMoveAt g).s.history.length := by
+--   simp [playAMoveAt]; split_ifs <;> simp
+-- 
+-- @[simp]
+-- theorem Game.length_history_le_playDMoveAt {pw} {g : Game pw} {h} :
+-- g.s.history.length ≤ (playDMoveAt g h).s.history.length := by
+--   simp [playDMoveAt]
+-- 
+-- @[simp]
+-- theorem Game.length_history_le_playMove {pw} {g : Game pw} :
+-- g.s.history.length ≤ g.playMove.s.history.length := by
+--   simp [playMove]
+--   split_ifs with h; on_goal 2 => rfl
+--   apply length_history_le_playAMoveAt.trans'
+--   simp
+-- 
+-- @[simp]
+-- theorem Game.length_history_le_play {pw} {g : Game pw} {n} :
+-- g.s.history.length ≤ (g.play n).s.history.length := by
+--   induction n generalizing g <;> simp; nm n ih
+--   apply length_history_le_playMove.trans' ih
+-- 
+-- theorem Game.length_hist_play_le_of_le {pw} {g : Game pw} {k n}
+-- (h : k ≤ n) : (g.play k).s.history.length ≤ (g.play n).s.history.length := by
+--   obtain ⟨n, rfl⟩ := Nat.exists_eq_add_of_le h; simp
+-- 
+-- @[simp]
+-- theorem Game.length_hist_lt_playMove_iff_act {pw} {g : Game pw} :
+-- g.s.history.length < g.playMove.s.history.length ↔ g.s.act := by
+--   constructor
+--   · contrapose!; intro h
+--     rw [playMove_eq_of_not_act h]
+--   intro h
+--   simp [playMove, h]
+--   apply lt_of_lt_of_le (b := playDMoveAt g h |>.s.history.length)
+--   · simp
+--   · simp only [length_history_le_playAMoveAt]
+-- 
+-- theorem Game.length_hist_play_lt_of_lt_and_act {pw} {g : Game pw} {k n}
+-- (h₁ : k < n) (h₂ : (g.play k).act) :
+-- (g.play k).s.history.length < (g.play n).s.history.length := by
+--   rw [←Nat.add_one_le_iff] at h₁ ⊢
+--   obtain ⟨n, rfl⟩ := Nat.exists_eq_add_of_le h₁; clear h₁
+--   simp only [play_add, play_succ]
+--   apply length_history_le_play.trans'; simpa
+-- 
+-- @[simp]
+-- theorem Game.setState_inj {pw} {g : Game pw} {s₁ s₂} :
+-- g.setState s₁ = g.setState s₂ ↔ s₁ = s₂ := by
+--   simp [setState]
+-- 
+-- @[simp]
+-- theorem A.f_set_of_eq {pw} {a a₀ : A pw} {s} : (a.set s a₀).f s = a₀.f s := by
+--   simp [set]
+-- 
+-- @[simp]
+-- theorem D.f_set_of_eq {d d₀ : D} {s} : (d.set s d₀).f s = d₀.f s := by
+--   simp [set]
+-- 
+-- @[simp]
+-- theorem Game.playAMoveAt'_set_of_eq {pw} {g : Game pw} {a a₀ : A pw} {h₁ h₂} :
+-- playAMoveAt' (a.set g.s a₀) g h₁ h₂ = playAMoveAt' a₀ g h₁ h₂ := by
+--   simp [playAMoveAt']
+-- 
+-- @[simp]
+-- theorem Game.playAMoveAt_initGame_a_set_of_eq {pw} {a a₀ : A pw} {d s} :
+-- (playAMoveAt # initGame (a.set s a₀) d s).s = (playAMoveAt # initGame a₀ d s).s := by
+--   simp [playAMoveAt]
+--   split_ifs with h; on_goal 2 => rfl
+--   simp [playAMoveAt']
+-- 
+-- @[simp]
+-- theorem Game.playDMoveAt_initGame_d_set_of_eq {pw} {a : A pw} {d d₀ : D} {s} {h} :
+-- (playDMoveAt (initGame a (d.set s d₀) s) h).s = (playDMoveAt (initGame a d₀ s) h).s := by
+--   simp
+-- 
+-- @[simp] theorem Game.initGame_self {pw} {g : Game pw} : initGame g.a g.d g.s = g := rfl
+-- theorem Game.eq_initGame {pw} {g : Game pw} : g = initGame g.a g.d g.s := rfl
+-- 
+-- @[simp]
+-- theorem Game.s_playAMoveAt_congr {pw} {g : Game pw} {d} :
+-- (playAMoveAt # initGame g.a d g.s).s = (playAMoveAt g).s := by
+--   simp [playAMoveAt]; split_ifs <;> tauto
+-- 
+-- @[simp]
+-- theorem Game.s_playDMoveAt_congr {pw} {g : Game pw} {a} {h} :
+-- (playDMoveAt (initGame a g.d g.s) h).s = (playDMoveAt g h).s := by
+--   simp
+-- 
+-- theorem Game.wf_playAMoveAt {pw} {g : Game pw} [hs : State.WF pw g.s]
+-- (h : g.s.aTurn) : State.WF pw (playAMoveAt g).s := by
+--   obtain ⟨a, d, n, g₁, h₁, h₂ | ⟨h₂, h₃⟩⟩ := id hs
+--   · rw [←h₂, ←h₁] at h
+--     rw [aTurn_play_iff (by simp) (by simp)] at h
+--     simp at h
+--     have h₃ : ¬g.s.act
+--     · rwa [Game.act, ←h₂, ←h₁]
+--     rw [playAMoveAt_eq_of_neg (by tauto)]
+--     rwa [finish_eq_of_not_act h₃]
+--   have h₂' : g₁.act := h₂
+--   have h₄ : g.s.act
+--   · rw [Game.act, ←h₃, ←Game.act]
+--     simp
+--   generalize ha' : a.set g.s g.a = a'
+--   refine' ⟨a', d, n + 1, initGame a' d (playAMoveAt g).s, _, _⟩
+--   simp
+--   have H₂ : g₁.d = d; simp [←h₁]
+--   convert_to (initGame a' d g₁.s).playMove = _
+--   on_goal 3 => simp
+--   · subst ha'
+--     congr
+--     ext:1 <;> simp
+--     rw [←h₁]
+--     rw [s_play_initGame_a_set_eq_of_ne]
+--     intro k hk h₅
+--     apply ne_of_congr (·.history.length)
+--     simp [←h₃, ←h₁]
+--     apply ne_of_lt
+--     rw [←Nat.add_one_le_iff] at hk ⊢
+--     obtain ⟨n, rfl⟩ := Nat.exists_eq_add_of_le hk
+--     simp only [play_add, play_succ, Order.add_one_le_iff]
+--     apply length_history_le_play.trans'
 --     simpa
---   
---   obtain ⟨h₅, h₆⟩ : (g₁.s.toAltH pw).dHws ∧ g₁.s.dwn pw < s.dwn pw
+--   · ext:1 <;> simp
+--     subst ha'
+--     simp [playMove, h₂]
+--     simp [playDMoveAt, H₂] at h₃ ⊢
+--     simp [h₃]
+-- 
+-- theorem Game.wf_playDMoveAt {pw} {g : Game pw} [hs : State.WF pw g.s] {hh}
+-- (h : g.s.aTurn = false) : State.WF pw (playDMoveAt g hh).s := by
+--   obtain ⟨a, d, n, g₁, h₁, h₂ | ⟨h₂, h₃⟩⟩ := id hs
+--   rotate_left
 --   ·
---     clear ih
---     apply @dHws_and_dwn_lt_toAltH_playDMoveAt_dOptimal_of_dHws pw (initGame a d s) g₁
---     simp [h₂]; all_goals simpa
---   
---   have hs₁ : sys.WF # g₁.s.toAltH pw
+--     rw [←h₃] at h
+--     simp at h
+--     rw [←h₁] at h
+--     rw [aTurn_play_iff (by simp) (by simp)] at h
+--     simp [h₁] at h
+--     have h₃ : ¬g.s.act
+--     · rwa [Game.act, ←h₂, ←h₁]
+--     rw [playAMoveAt_eq_of_neg (by tauto)]
+--     rwa [finish_eq_of_not_act h₃]
 --   ·
---     clear ih
---     simp [←hg₁]
---   
---   -- specialize ih _ (by omega) g₁.s h₅ rfl hs₁ (by simpa [←hg₁])
+--     use a, d, n, g₁, h₁
+-- 
+-- #check 0 #exit
+-- 
+-- -- theorem State.invariant_of_wf {pw s} {p : State → Prop} [hs : WF pw s]
+-- -- (h₁ : p state₀) (h₄ : ∀ ⦃s⦄, WF pw s → p s → p s.finish)
+-- -- (h₂ : ∀ ⦃s m⦄, WF pw s → AMoveValid pw s.board m → p s → p (applyAMove s m))
+-- -- (h₃ : ∀ ⦃s m⦄, WF pw s → DMoveValid s.board m → p s → p (applyDMove s m)) : p s := by
+-- --   rw [wf_iff] at hs
+-- --   choose a d n g h₄ h₅ using hs
+-- --   induction n generalizing g s
+-- --   · simp at h₄
+-- --     subst h₄
+-- --     simp at h₅
+-- --     rcases h₅ with rfl | rfl
+-- --     · exact h₁
+-- --     apply h₃ (by simp) _ h₁
+-- --     exact d.f state₀ (by simp) |>.2
+-- --   nm n ih
+-- --   simp at h₄
+-- --   generalize hg : (initGame a d state₀).play n = g at h₄
+-- --   subst h₄
+-- --   specialize @ih g.s g hg
+-- --   simp at ih
+-- --   have h₆ : p g.playMove.s
+-- --   · simp [Game.playMove]
+-- --     split_ifs with h₆; on_goal 2 => exact ih
+-- --     generalize hs' : (playDMoveAt g h₆).s = s'
+-- --     rw [playAMoveAt]
+-- --     have hs : WF pw g.s
+-- --     ·
+-- --       use a, d, n, g, hg; simp
+-- --     have h₈ : p s'
+-- --     · subst hs'
+-- --       apply h₃ hs _ ih
+-- --       convert d.f g.s h₆ |>.2
+-- --       simp [←hg]
+-- --     have hs₁ : WF pw s'
+-- --     ·
+-- --       subst hs'
+-- --       sorry
+-- --     split_ifs with h₇
+-- --     rotate_left
+-- --     · subst hs'; exact h₄ hs₁ h₈
+-- --     rcases h₇ with ⟨h₇, h₉⟩
+-- --     apply h₂ (by rwa [hs']) _ (by rwa [hs'])
+-- --     simp [hs'] at h₉ ⊢
+-- --     rw [Game.act, hs'] at h₇
+-- --     rw! [hs']
+-- --     convert a.f s' h₇ h₉ |>.2
+-- --     simp [←hg]
+-- --   rcases h₅ with rfl | ⟨h₅, rfl⟩
+-- --   · exact h₆
+-- --   apply h₃ _ _ h₆
+-- --   ·
+-- --     sorry
+-- --   convert d.f _ _ |>.2
+-- --   · simp [←hg]
+-- --   · exact h₅
+-- -- 
+-- -- #check 0 #exit
+-- -- 
+-- -- theorem Board.invariant_of_wf {pw s} {p : Board → Prop} [hs : State.WF pw s] (h₁ : p board₀)
+-- -- (h₂ : ∀ ⦃b m⦄, AMoveValid pw b m → p b → p (applyAMoveB b m))
+-- -- (h₃ : ∀ ⦃b m⦄, DMoveValid b m → p b → p (applyDMoveB b m)) : p s.board := by
+-- --   apply s.invariant_of_wf <;> tauto
+-- -- 
+-- -- @[simp]
+-- -- theorem dMoveValid_some_iff {b p} : DMoveValid b (some p) ↔ p ≠ b.A ∧ p ∈ b.squares := by rfl
+-- -- 
+-- -- theorem dMoveValid_iff {b m} : DMoveValid b m ↔ m = none ∨
+-- -- ∃ p, m = some p ∧ p ≠ b.A ∧ p ∈ b.squares := by
+-- --   cases m <;> simp
+-- -- 
+-- -- @[simp] theorem Board.a_applyAMoveB {b m} : (applyAMoveB b m).A = m := rfl
+-- -- 
+-- -- @[simp] theorem Board.a_applyDMoveB {b m} : (applyDMoveB b m).A = b.A := by
+-- --   cases m <;> rfl
+-- -- 
+-- -- @[simp]
+-- -- theorem Board.squares_applyAMoveB {b m} : (applyAMoveB b m).squares = b.squares := rfl
+-- -- 
+-- -- @[simp]
+-- -- theorem Board.squares_applyDMoveB {b m} :
+-- -- (applyDMoveB b m).squares = b.squares \ m.elim ∅ ({·}) := by
+-- --   cases m <;> simp [applyDMoveB]
+-- -- 
+-- -- theorem State.a_mem_squares_of_wf {pw s} [hs : WF pw s] : s.board.A ∈ s.board.squares := by
+-- --   apply Board.invariant_of_wf (p := λ b => b.A ∈ b.squares) <;> clear! s; simp
+-- --   · simp [AMoveValid]; tauto
+-- --   · intro b m h₁ h₂
+-- --     simp [dMoveValid_iff] at h₁
+-- --     simp
+-- --     cases m <;> simp_all
+-- --     tauto
+-- -- 
+-- -- @[simp]
+-- -- theorem squares_board_applyAMove {s m} :
+-- -- (applyAMove s m).board.squares = s.board.squares := rfl
+-- -- 
+-- -- -- #check 0 #exit
+-- -- 
+-- -- theorem State.exi_toAlt_board_not_aTurn_of_dState {pw s} [hs : DState pw s] :
+-- -- ∃ s₁, sys.WF s₁ ∧ s.board.toAlt pw false s₁.hist = s₁ := by
+-- --   cases hs; nm hs ht
+-- --   apply exi_wf_toAlt_board_of_wfCnd
+-- --   constructor <;> simp; exact a_mem_squares_of_wf
+-- --   simp [Set'.eq_empty_iff]
+-- --   intro p hp
+-- --   simp [AP.State.aMove]
+-- --   revert p ht hp
+-- --   apply s.invariant_of_wf; iterate 2 simp
+-- --   all_goals clear! s; intro s m h₁ h₂ ht p hp
+-- --   ·
+-- --     -- simp [applyAMove] at ht hp ⊢
+-- --     simp [applyAMove]
+-- --     choose h₁ h₃ h₄ using h₁
+-- --     use s.board.A.toAlt
+-- --     simp [h₁]
+-- -- 
+-- -- #check 0 #exit
+-- -- 
+-- -- -- theorem State.exi_toAlt_board_of_dState {pw s t} [hs : DState pw s] :
+-- -- -- ∃ s₁, sys.WF s₁ ∧ s.board.toAlt pw t s₁.hist = s₁ := by
+-- -- 
+-- -- -- #check 0 #exit
+-- -- 
+-- -- -- theorem Game.toAltH_playDMoveAt_of_none {pw} {g : Game pw} {h} [hs : DState pw g.s]
+-- -- -- (h₁ : (g.d.f g.s h).m = none) : ∃ hist,
+-- -- -- (playDMoveAt g h).s.toAltH pw = g.s.toAlt pw hist := by
+-- -- --   simp [playDMoveAt, applyDMove, applyDMoveB, h₁, applyMove,State.toAltH,
+-- -- --     State.toAltH?, State.toAlt]
+-- -- --   
+-- -- --   congr 1
+-- -- --   apply Board.getd_toAltH?_eq_toAlt_of
+-- -- --   simp_rw [State.toAlt_eq]
+-- -- 
+-- -- -- #check 0 #exit
+-- -- 
+-- -- -- theorem dHws_and_dwn_lt_toAltH_playDMoveAt_dOptimal_of_dHws {pw} {g g₁ : Game pw} {h}
+-- -- -- [hs : DState pw g.s]
+-- -- -- (h₁ : g.d = (dOptimal pw).getd)
+-- -- -- (h₂ : g.s.toAltH pw |>.dHws)
+-- -- -- (hg₁ : playDMoveAt g h = g₁) :
+-- -- -- (g₁.s.toAltH pw).dHws ∧ g₁.s.dwn pw < g.s.dwn pw := by
+-- -- --   split_ands
+-- -- --   ·
+-- -- --     simp [←hg₁]
+-- -- -- 
+-- -- -- #check 0 #exit
+-- -- -- 
+-- -- -- theorem DHws_of_alt {pw} (h : AP.dHwsPw pw) : DHws pw := by
+-- -- --   specialize h 0
+-- -- --   generalize h₀ : state₀ = s
+-- -- --   
+-- -- --   replace h : s.toAltH pw |>.dHws
+-- -- --   ·
+-- -- --     subst h₀
+-- -- --     simp [State.toAltH, State.toAltH?, Board.toAltH?]
+-- -- --     
+-- -- --     apply choose?_of_pos (P := λ (x : Option AP.State) => x.getd.dHws) _ _
+-- -- --     ·
+-- -- --       use AP.initState pw 0
+-- -- --       simp
+-- -- --     
+-- -- --     rintro s - ⟨hs, h₂⟩
+-- -- --     simp at h₂ ⊢
+-- -- --     rw [setHist_eq_comm] at h₂
+-- -- --     simp at h₂
+-- -- --     rw [←h₂] at h
+-- -- --     
+-- -- --     have h₁ : sys.WF # s.setHist [0]
+-- -- --     ·
+-- -- --       simp [h₂]
+-- -- --     
+-- -- --     simp at h
+-- -- --     exact h
+-- -- --   
+-- -- --   have h₁ : s.toAltH pw = AP.initState pw 0
+-- -- --   ·
+-- -- --     simp [←h₀]
+-- -- --   
+-- -- --   generalize hn : s.dwn pw = n
+-- -- --   generalize h₂ : (dOptimal pw).getd = d
+-- -- --   use d
+-- -- --   intro a
+-- -- --   have hs : sys.WF # s.toAltH pw; simp [h₁]
+-- -- --   
+-- -- --   rw [h₀]
+-- -- --   have h₃ : s.act
+-- -- --   ·
+-- -- --     rw [←h₀]
+-- -- --     simp
+-- -- --   
+-- -- --   have ht : s.aTurn = false
+-- -- --   ·
+-- -- --     simp [←h₀]
+-- -- --   
+-- -- --   clear h₀ h₁
+-- -- --   
+-- -- --   use n
+-- -- --   
+-- -- --   induction n using Nat.strong_induction_on generalizing s
+-- -- --   nm n ih
+-- -- --   cases n
+-- -- --   ·
+-- -- --     contrapose! hn
+-- -- --     simpa [State.dwn_eq, State.dwn_eq_zero_iff_aHws]
+-- -- --   nm n
+-- -- --   simp at ih
+-- -- --   
+-- -- --   rw [Game.play_succ', Game.playMove]
+-- -- --   simp [h₃, playAMoveAt]
+-- -- --   rw! [eq_true_of Game.act_playDMoveAt]
+-- -- --   rw! (castMode := .all) [true_and]
+-- -- --   
+-- -- --   split_ifs with h₄
+-- -- --   on_goal 2 => simp
+-- -- --   
+-- -- --   generalize_proofs H₁ H₂ H₃
+-- -- --   by_contra H
+-- -- --   generalize hg₁ : playDMoveAt (initGame a d s) H₁ = g₁
+-- -- --   contrapose H; clear H
+-- -- --   rw! [hg₁] at h₄ ⊢
+-- -- --   
+-- -- --   have ht₁ : g₁.s.aTurn = true
+-- -- --   ·
+-- -- --     clear ih
+-- -- --     subst hg₁
+-- -- --     simpa
+-- -- --   
+-- -- --   obtain ⟨h₅, h₆⟩ : (g₁.s.toAltH pw).dHws ∧ g₁.s.dwn pw < s.dwn pw
+-- -- --   ·
+-- -- --     clear ih
+-- -- --     apply @dHws_and_dwn_lt_toAltH_playDMoveAt_dOptimal_of_dHws pw (initGame a d s) g₁
+-- -- --     simp [h₂]; all_goals simpa
+-- -- --   
+-- -- --   have hs₁ : sys.WF # g₁.s.toAltH pw
+-- -- --   ·
+-- -- --     clear ih
+-- -- --     simp [←hg₁]
+-- -- --   
+-- -- --   -- specialize ih _ (by omega) g₁.s h₅ rfl hs₁ (by simpa [←hg₁])
+-- -- 
+-- -- -- theorem Game.toAltH_playDMoveAt {pw} {g : Game pw} {h} [hs : DState pw g.s] :
+-- -- -- ∃ hist s', (g.s.toAltH pw).dMove (Point.toAlt # g.d.f g.s h) = some s' ∧
+-- -- -- (playDMoveAt g h).s.toAltH pw = s'.setHist hist
+-- -- -- 
+-- -- -- #check 0 #exit
+-- -- 
+-- -- -- @[simp, instance]
+-- -- -- theorem State.wf_toAltH {pw} {s : State} [hs : s.WF pw] : sys.WF # s.toAltH pw := by
+-- -- --   rw [wf_iff] at hs
+-- -- --   choose a d n g h₁ h₂ using hs
+-- -- --   induction n generalizing g
+-- -- --   ·
+-- -- --     simp at h₁
+-- -- --     simp [←h₁] at h₂
+-- -- --     rcases h₂ with rfl | ⟨h', h₂⟩; simp
+-- -- 
+-- -- -- @[simp]
+-- -- -- theorem State.pw_toAltH {pw} {s : State} : (s.toAltH pw).pw = pw := by
+-- -- --   unfold toAltH toAltH? Board.toAltH?
